rename

theory/Sound_Semantics.thy
@@ -15,8 +15,8 @@ definition env_to_abstract_value_env :: "(var \<rightharpoonup> val) \<Rightarro
     None \<Rightarrow> {}
   ))"
 
-inductive accept_value :: "abstract_value_env \<times> abstract_value_env \<Rightarrow> val \<Rightarrow> bool" (infix "\<Turnstile>\<^sub>\<omega>" 55)
-and  accept_val_env :: "abstract_value_env \<times> abstract_value_env \<Rightarrow> val_env \<Rightarrow> bool" (infix "\<Turnstile>\<^sub>\<rho>" 55) 
+inductive static_eval_value :: "abstract_value_env \<times> abstract_value_env \<Rightarrow> val \<Rightarrow> bool" (infix "\<Turnstile>\<^sub>\<omega>" 55)
+and  static_eval_env :: "abstract_value_env \<times> abstract_value_env \<Rightarrow> val_env \<Rightarrow> bool" (infix "\<Turnstile>\<^sub>\<rho>" 55) 
 where
   Unit: "
     (\<V>, \<C>) \<Turnstile>\<^sub>\<omega> \<lbrace>\<rbrace>
@@ -75,7 +75,7 @@ where
   "
 
 
-inductive accept_stack :: "abstract_value_env \<times> abstract_value_env \<Rightarrow> abstract_value set \<Rightarrow> cont list \<Rightarrow> bool" ("_ \<Turnstile>\<^sub>\<kappa> _ \<Rrightarrow> _" [56,0,56]55) where
+inductive static_eval_stack :: "abstract_value_env \<times> abstract_value_env \<Rightarrow> abstract_value set \<Rightarrow> cont list \<Rightarrow> bool" ("_ \<Turnstile>\<^sub>\<kappa> _ \<Rrightarrow> _" [56,0,56]55) where
   Empty: "(\<V>, \<C>) \<Turnstile>\<^sub>\<kappa> \<W> \<Rrightarrow> []" |
   Nonempty: "
     \<lbrakk> 
@@ -98,7 +98,7 @@ inductive accept_state :: "abstract_value_env \<times> abstract_value_env \<Righ
     (\<V>, \<C>) \<Turnstile>\<^sub>\<sigma> \<langle>e; \<rho>; \<kappa>\<rangle>
   "
 
-inductive accept_state_pool :: "abstract_value_env \<times> abstract_value_env \<Rightarrow> state_pool \<Rightarrow> bool" (infix "\<Turnstile>\<^sub>\<E>" 55) where
+inductive static_eval_pool :: "abstract_value_env \<times> abstract_value_env \<Rightarrow> trace_pool \<Rightarrow> bool" (infix "\<Turnstile>\<^sub>\<E>" 55) where
   Any: "
     (\<forall> \<pi> \<sigma> . \<E> \<pi> = Some \<sigma> \<longrightarrow> (\<V>, \<C>) \<Turnstile>\<^sub>\<sigma> \<sigma>)
     \<Longrightarrow> 
@@ -111,7 +111,7 @@ lemma accept_state_to_exp_result: "
 proof -
  assume "(\<V>, \<C>) \<Turnstile>\<^sub>\<sigma> \<langle>RESULT x;\<rho>;\<langle>x\<^sub>\<kappa>,e\<^sub>\<kappa>,\<rho>\<^sub>\<kappa>\<rangle> # \<kappa>\<rangle>" then
  have "(\<V>, \<C>) \<Turnstile>\<^sub>\<kappa> \<V> x \<Rrightarrow> \<langle>x\<^sub>\<kappa>,e\<^sub>\<kappa>,\<rho>\<^sub>\<kappa>\<rangle> # \<kappa>" by (simp add: accept_state.simps) then
- show "(\<V>, \<C>) \<Turnstile>\<^sub>e e\<^sub>\<kappa>" by (rule accept_stack.cases; auto)
+ show "(\<V>, \<C>) \<Turnstile>\<^sub>e e\<^sub>\<kappa>" by (rule static_eval_stack.cases; auto)
 qed
 
 
@@ -126,7 +126,7 @@ proof -
   have "(\<V>, \<C>) \<Turnstile>\<^sub>e LET x = CASE x\<^sub>s LEFT x\<^sub>l |> e\<^sub>l RIGHT x\<^sub>r |> e\<^sub>r in e"  
   and "(\<V>, \<C>) \<Turnstile>\<^sub>\<rho> \<rho>"
   by (simp add: accept_state.simps)+ then
-  have "\<forall>x \<omega>. \<rho> x = Some \<omega> \<longrightarrow> {|\<omega>|} \<subseteq> \<V> x" by (simp add: accept_val_env.simps)
+  have "\<forall>x \<omega>. \<rho> x = Some \<omega> \<longrightarrow> {|\<omega>|} \<subseteq> \<V> x" by (simp add: static_eval_env.simps)
   with `\<rho> x\<^sub>s = Some \<lbrace>prim.Left x\<^sub>l', \<rho>\<^sub>l\<rbrace>`
   have "^prim.Left x\<^sub>l' \<in> \<V> x\<^sub>s" by fastforce
   with `(\<V>, \<C>) \<Turnstile>\<^sub>e LET x = CASE x\<^sub>s LEFT x\<^sub>l |> e\<^sub>l RIGHT x\<^sub>r |> e\<^sub>r in e`
@@ -152,7 +152,7 @@ proof -
   have "(\<V>, \<C>) \<Turnstile>\<^sub>e LET x = CASE x\<^sub>s LEFT x\<^sub>l |> e\<^sub>l RIGHT x\<^sub>r |> e\<^sub>r in e"  
   and "(\<V>, \<C>) \<Turnstile>\<^sub>\<rho> \<rho>" 
     by (simp add: accept_state.simps)+ then
-  have "\<forall>x \<omega>. \<rho> x = Some \<omega> \<longrightarrow> {|\<omega>|} \<subseteq> \<V> x" by (simp add: accept_val_env.simps)
+  have "\<forall>x \<omega>. \<rho> x = Some \<omega> \<longrightarrow> {|\<omega>|} \<subseteq> \<V> x" by (simp add: static_eval_env.simps)
   with `\<rho> x\<^sub>s = Some \<lbrace>prim.Right x\<^sub>r', \<rho>\<^sub>r\<rbrace>`
   have "^prim.Right x\<^sub>r' \<in> \<V> x\<^sub>s" by fastforce
   with `(\<V>, \<C>) \<Turnstile>\<^sub>e LET x = CASE x\<^sub>s LEFT x\<^sub>l |> e\<^sub>l RIGHT x\<^sub>r |> e\<^sub>r in e`
@@ -173,7 +173,7 @@ lemma accept_state_to_exp_let: "
 proof -
  assume "(\<V>, \<C>) \<Turnstile>\<^sub>\<sigma> \<langle>LET x = b in e; \<rho>; \<kappa>\<rangle>" then
  have "(\<V>, \<C>) \<Turnstile>\<^sub>e LET x = b in e" by (simp add: accept_state.simps) then
- show "(\<V>, \<C>) \<Turnstile>\<^sub>e e" by (rule accept_exp.cases; auto)
+ show "(\<V>, \<C>) \<Turnstile>\<^sub>e e" by (rule static_eval.cases; auto)
 qed
 
 
@@ -187,10 +187,10 @@ proof -
   assume "\<rho> f = Some \<lbrace>Abs f' x\<^sub>p e\<^sub>b, \<rho>'\<rbrace>"
   assume "(\<V>, \<C>) \<Turnstile>\<^sub>\<sigma> \<langle>LET x = APP f x\<^sub>a in e; \<rho>; \<kappa>\<rangle>" then
   have "(\<V>, \<C>) \<Turnstile>\<^sub>\<rho> \<rho>" by (simp add: accept_state.simps) then
-  have "\<forall>x \<omega>. \<rho> x = Some \<omega> \<longrightarrow> {|\<omega>|} \<subseteq> \<V> x \<and> (\<V>, \<C>) \<Turnstile>\<^sub>\<omega> \<omega>" by (simp add: accept_val_env.simps)
+  have "\<forall>x \<omega>. \<rho> x = Some \<omega> \<longrightarrow> {|\<omega>|} \<subseteq> \<V> x \<and> (\<V>, \<C>) \<Turnstile>\<^sub>\<omega> \<omega>" by (simp add: static_eval_env.simps)
   with `\<rho> f = Some \<lbrace>Abs f' x\<^sub>p e\<^sub>b, \<rho>'\<rbrace>`
   have "(\<V>, \<C>) \<Turnstile>\<^sub>\<omega> \<lbrace>Abs f' x\<^sub>p e\<^sub>b, \<rho>'\<rbrace>" by simp then
-  show "(\<V>, \<C>) \<Turnstile>\<^sub>e e\<^sub>b" by (rule accept_value.cases; auto)
+  show "(\<V>, \<C>) \<Turnstile>\<^sub>e e\<^sub>b" by (rule static_eval_value.cases; auto)
 qed
 
 lemma accept_state_to_env_result: "
@@ -205,7 +205,7 @@ proof
  have "(\<V>, \<C>) \<Turnstile>\<^sub>\<kappa> \<V> x \<Rrightarrow> \<langle>x\<^sub>\<kappa>,e\<^sub>\<kappa>,\<rho>\<^sub>\<kappa>\<rangle> # \<kappa>" and "(\<V>, \<C>) \<Turnstile>\<^sub>\<rho> \<rho>" by (rule accept_state.cases; auto)+
 
  from `(\<V>, \<C>) \<Turnstile>\<^sub>\<rho> \<rho>` and `\<rho> x = Some \<omega>`
- have "{|\<omega>|} \<subseteq> \<V> x" "(\<V>, \<C>) \<Turnstile>\<^sub>\<omega> \<omega>" by (simp add: accept_val_env.simps)+
+ have "{|\<omega>|} \<subseteq> \<V> x" "(\<V>, \<C>) \<Turnstile>\<^sub>\<omega> \<omega>" by (simp add: static_eval_env.simps)+
 
  from `(\<V>, \<C>) \<Turnstile>\<^sub>\<kappa> \<V> x \<Rrightarrow> \<langle>x\<^sub>\<kappa>,e\<^sub>\<kappa>,\<rho>\<^sub>\<kappa>\<rangle> # \<kappa>`
  show "\<forall>x \<omega>'. (\<rho>\<^sub>\<kappa>(x\<^sub>\<kappa> \<mapsto> \<omega>)) x = Some \<omega>' \<longrightarrow> {|\<omega>'|} \<subseteq> \<V> x \<and> (\<V>, \<C>) \<Turnstile>\<^sub>\<omega> \<omega>'"
@@ -232,7 +232,7 @@ proof
        have "\<rho>\<^sub>\<kappa> x' = Some \<omega>'" by simp 
        with `(\<V>, \<C>) \<Turnstile>\<^sub>\<rho> \<rho>\<^sub>\<kappa>`
        
-       show "{|\<omega>'|} \<subseteq> \<V> x' \<and> (\<V>, \<C>) \<Turnstile>\<^sub>\<omega> \<omega>'" by (simp add: accept_val_env.simps)+
+       show "{|\<omega>'|} \<subseteq> \<V> x' \<and> (\<V>, \<C>) \<Turnstile>\<^sub>\<omega> \<omega>'" by (simp add: static_eval_env.simps)+
      qed
    } then
 
@@ -250,7 +250,7 @@ proof -
   assume "\<rho> x = Some \<omega>"
   assume "(\<V>, \<C>) \<Turnstile>\<^sub>\<sigma> \<langle>RESULT x; \<rho>; \<langle>x\<^sub>\<kappa>,e\<^sub>\<kappa>,\<rho>\<^sub>\<kappa>\<rangle> # \<kappa>\<rangle>" then
   have "(\<V>, \<C>) \<Turnstile>\<^sub>\<kappa> \<V> x \<Rrightarrow> \<langle>x\<^sub>\<kappa>,e\<^sub>\<kappa>,\<rho>\<^sub>\<kappa>\<rangle> # \<kappa>" by (simp add: accept_state.simps) then
-  show "(\<V>, \<C>) \<Turnstile>\<^sub>\<kappa> \<V> (\<lfloor>e\<^sub>\<kappa>\<rfloor>) \<Rrightarrow> \<kappa>" by (rule accept_stack.cases; auto)
+  show "(\<V>, \<C>) \<Turnstile>\<^sub>\<kappa> \<V> (\<lfloor>e\<^sub>\<kappa>\<rfloor>) \<Rrightarrow> \<kappa>" by (rule static_eval_stack.cases; auto)
 qed
 
 
@@ -279,7 +279,7 @@ proof
   have "(\<V>, \<C>) \<Turnstile>\<^sub>e LET x = \<lparr>\<rparr> in e" "(\<V>, \<C>) \<Turnstile>\<^sub>\<rho> \<rho>" by (simp add: accept_state.simps)+ 
 
   from `(\<V>, \<C>) \<Turnstile>\<^sub>e LET x = \<lparr>\<rparr> in e`
-  have "{^\<lparr>\<rparr>} \<subseteq> \<V> x" by (rule accept_exp.cases; auto)+
+  have "{^\<lparr>\<rparr>} \<subseteq> \<V> x" by (rule static_eval.cases; auto)+
   have "(\<V>, \<C>) \<Turnstile>\<^sub>\<omega> \<lbrace>\<rbrace>" by (simp add: Unit)
 
   {
@@ -299,7 +299,7 @@ proof
 
       from `(\<V>, \<C>) \<Turnstile>\<^sub>\<rho> \<rho>` `\<rho> x' = Some \<omega>'`
 
-      show "{|\<omega>'|} \<subseteq> \<V> x' \<and> (\<V>, \<C>) \<Turnstile>\<^sub>\<omega> \<omega>'" by (simp add: accept_val_env.simps)
+      show "{|\<omega>'|} \<subseteq> \<V> x' \<and> (\<V>, \<C>) \<Turnstile>\<^sub>\<omega> \<omega>'" by (simp add: static_eval_env.simps)
     qed
 
   }
@@ -328,10 +328,10 @@ proof
 
 qed
 
-lemma accept_exp_to_value_let_prim: "
+lemma static_eval_to_value_let_prim: "
   (\<V>, \<C>) \<Turnstile>\<^sub>e LET x = Prim p in e \<Longrightarrow> (\<V>, \<C>) \<Turnstile>\<^sub>\<rho> \<rho> \<Longrightarrow> (\<V>, \<C>) \<Turnstile>\<^sub>\<omega> \<lbrace>p, \<rho>\<rbrace>
 "
-by (erule accept_exp.cases; auto; rule; auto)
+by (erule static_eval.cases; auto; rule; auto)
 
 lemma accept_state_to_env_let_prim: "
   (\<V>, \<C>) \<Turnstile>\<^sub>\<sigma> \<langle>LET x = Prim p in e; \<rho>; \<kappa>\<rangle> \<Longrightarrow> (\<V>, \<C>) \<Turnstile>\<^sub>\<rho> \<rho>(x \<mapsto> \<lbrace>p, \<rho>\<rbrace>)
@@ -339,10 +339,10 @@ lemma accept_state_to_env_let_prim: "
 proof
   assume "(\<V>, \<C>) \<Turnstile>\<^sub>\<sigma> \<langle>LET x = Prim p in e; \<rho>; \<kappa>\<rangle> " then 
   have "(\<V>, \<C>) \<Turnstile>\<^sub>e LET x = Prim p in e" "(\<V>, \<C>) \<Turnstile>\<^sub>\<rho> \<rho>" by (simp add: accept_state.simps)+ then
-  have "(\<V>, \<C>) \<Turnstile>\<^sub>\<omega> \<lbrace>p, \<rho>\<rbrace>" by (simp add: accept_exp_to_value_let_prim)
+  have "(\<V>, \<C>) \<Turnstile>\<^sub>\<omega> \<lbrace>p, \<rho>\<rbrace>" by (simp add: static_eval_to_value_let_prim)
 
   from `(\<V>, \<C>) \<Turnstile>\<^sub>e LET x = Prim p in e`
-  have "{^p} \<subseteq> \<V> x" by (rule accept_exp.cases; auto)+
+  have "{^p} \<subseteq> \<V> x" by (rule static_eval.cases; auto)+
  
   {
     fix x' \<omega>'
@@ -359,7 +359,7 @@ proof
       have "\<rho> x' = Some \<omega>'" by simp
       with `(\<V>, \<C>) \<Turnstile>\<^sub>\<rho> \<rho>` 
   
-      show "{|\<omega>'|} \<subseteq> \<V> x' \<and> (\<V>, \<C>) \<Turnstile>\<^sub>\<omega> \<omega>'" by (simp add: accept_val_env.simps)
+      show "{|\<omega>'|} \<subseteq> \<V> x' \<and> (\<V>, \<C>) \<Turnstile>\<^sub>\<omega> \<omega>'" by (simp add: static_eval_env.simps)
     qed
 
   } then
@@ -395,14 +395,14 @@ proof
   have "(\<V>, \<C>) \<Turnstile>\<^sub>e LET x = CASE x\<^sub>s LEFT x\<^sub>l |> e\<^sub>l RIGHT x\<^sub>r |> e\<^sub>r in e" "(\<V>, \<C>) \<Turnstile>\<^sub>\<rho> \<rho>" by (simp add: accept_state.simps)+
 
   from `(\<V>, \<C>) \<Turnstile>\<^sub>\<rho> \<rho>` `\<rho> x\<^sub>s = Some \<lbrace>prim.Left x\<^sub>l', \<rho>\<^sub>l\<rbrace>`
-  have "(\<V>, \<C>) \<Turnstile>\<^sub>\<omega> \<lbrace>prim.Left x\<^sub>l', \<rho>\<^sub>l\<rbrace>" by (blast intro: accept_val_env.cases) then
-  have "(\<V>, \<C>) \<Turnstile>\<^sub>\<rho> \<rho>\<^sub>l" by (blast intro: accept_value.cases)
+  have "(\<V>, \<C>) \<Turnstile>\<^sub>\<omega> \<lbrace>prim.Left x\<^sub>l', \<rho>\<^sub>l\<rbrace>" by (blast intro: static_eval_env.cases) then
+  have "(\<V>, \<C>) \<Turnstile>\<^sub>\<rho> \<rho>\<^sub>l" by (blast intro: static_eval_value.cases)
 
   from `(\<V>, \<C>) \<Turnstile>\<^sub>\<rho> \<rho>\<^sub>l` `\<rho>\<^sub>l x\<^sub>l' = Some \<omega>\<^sub>l`
-  have "{|\<omega>\<^sub>l|} \<subseteq> \<V> x\<^sub>l'" "(\<V>, \<C>) \<Turnstile>\<^sub>\<omega> \<omega>\<^sub>l" by (blast intro: accept_val_env.cases)+
+  have "{|\<omega>\<^sub>l|} \<subseteq> \<V> x\<^sub>l'" "(\<V>, \<C>) \<Turnstile>\<^sub>\<omega> \<omega>\<^sub>l" by (blast intro: static_eval_env.cases)+
 
   from `(\<V>, \<C>) \<Turnstile>\<^sub>\<rho> \<rho>` `\<rho> x\<^sub>s = Some \<lbrace>prim.Left x\<^sub>l', \<rho>\<^sub>l\<rbrace>`
-  have " | \<lbrace>prim.Left x\<^sub>l', \<rho>\<^sub>l\<rbrace> | \<in> \<V> x\<^sub>s" by (blast intro: accept_val_env.cases) then
+  have " | \<lbrace>prim.Left x\<^sub>l', \<rho>\<^sub>l\<rbrace> | \<in> \<V> x\<^sub>s" by (blast intro: static_eval_env.cases) then
   have "^prim.Left x\<^sub>l' \<in> \<V> x\<^sub>s" by simp
 
   from  `(\<V>, \<C>) \<Turnstile>\<^sub>e LET x = CASE x\<^sub>s LEFT x\<^sub>l |> e\<^sub>l RIGHT x\<^sub>r |> e\<^sub>r in e`
@@ -422,7 +422,7 @@ proof
     assume "(\<rho>(x\<^sub>l \<mapsto> \<omega>\<^sub>l)) x' = Some \<omega>'" "x' \<noteq> x\<^sub>l" then
     have "\<rho> x' = Some \<omega>'" by simp
     with `(\<V>, \<C>) \<Turnstile>\<^sub>\<rho> \<rho>` 
-    have "{|\<omega>'|} \<subseteq> \<V> x' \<and> (\<V>, \<C>) \<Turnstile>\<^sub>\<omega> \<omega>'" by (simp add: accept_val_env.simps)
+    have "{|\<omega>'|} \<subseteq> \<V> x' \<and> (\<V>, \<C>) \<Turnstile>\<^sub>\<omega> \<omega>'" by (simp add: static_eval_env.simps)
    
   }
   with `{|\<omega>\<^sub>l|} \<subseteq> \<V> x\<^sub>l` `(\<V>, \<C>) \<Turnstile>\<^sub>\<omega> \<omega>\<^sub>l`
@@ -444,7 +444,7 @@ proof
   have "(\<V>, \<C>) \<Turnstile>\<^sub>e LET x = CASE x\<^sub>s LEFT x\<^sub>l |> e\<^sub>l RIGHT x\<^sub>r |> e\<^sub>r in e" "(\<V>, \<C>) \<Turnstile>\<^sub>\<rho> \<rho>" by (blast intro: accept_state.cases)+
   
   from `(\<V>, \<C>) \<Turnstile>\<^sub>\<rho> \<rho>` `\<rho> x\<^sub>s = Some \<lbrace>prim.Left x\<^sub>l', \<rho>\<^sub>l\<rbrace>`
-  have " | \<lbrace>prim.Left x\<^sub>l', \<rho>\<^sub>l\<rbrace> | \<in> \<V> x\<^sub>s" by (blast intro: accept_val_env.cases) then
+  have " | \<lbrace>prim.Left x\<^sub>l', \<rho>\<^sub>l\<rbrace> | \<in> \<V> x\<^sub>s" by (blast intro: static_eval_env.cases) then
   have "^prim.Left x\<^sub>l' \<in> \<V> x\<^sub>s" by simp
 
   from `(\<V>, \<C>) \<Turnstile>\<^sub>e LET x = CASE x\<^sub>s LEFT x\<^sub>l |> e\<^sub>l RIGHT x\<^sub>r |> e\<^sub>r in e`
@@ -501,14 +501,14 @@ proof
   have "(\<V>, \<C>) \<Turnstile>\<^sub>e LET x = CASE x\<^sub>s LEFT x\<^sub>l |> e\<^sub>l RIGHT x\<^sub>r |> e\<^sub>r in e" "(\<V>, \<C>) \<Turnstile>\<^sub>\<rho> \<rho>" by (simp add: accept_state.simps)+
 
   from `(\<V>, \<C>) \<Turnstile>\<^sub>\<rho> \<rho>` `\<rho> x\<^sub>s = Some \<lbrace>prim.Right x\<^sub>r', \<rho>\<^sub>r\<rbrace>`
-  have "(\<V>, \<C>) \<Turnstile>\<^sub>\<omega> \<lbrace>prim.Right x\<^sub>r', \<rho>\<^sub>r\<rbrace>" by (blast intro: accept_val_env.cases) then
-  have "(\<V>, \<C>) \<Turnstile>\<^sub>\<rho> \<rho>\<^sub>r" by (blast intro: accept_value.cases)
+  have "(\<V>, \<C>) \<Turnstile>\<^sub>\<omega> \<lbrace>prim.Right x\<^sub>r', \<rho>\<^sub>r\<rbrace>" by (blast intro: static_eval_env.cases) then
+  have "(\<V>, \<C>) \<Turnstile>\<^sub>\<rho> \<rho>\<^sub>r" by (blast intro: static_eval_value.cases)
 
   from `(\<V>, \<C>) \<Turnstile>\<^sub>\<rho> \<rho>\<^sub>r` `\<rho>\<^sub>r x\<^sub>r' = Some \<omega>\<^sub>r`
-  have "{|\<omega>\<^sub>r|} \<subseteq> \<V> x\<^sub>r'" "(\<V>, \<C>) \<Turnstile>\<^sub>\<omega> \<omega>\<^sub>r" by (blast intro: accept_val_env.cases)+
+  have "{|\<omega>\<^sub>r|} \<subseteq> \<V> x\<^sub>r'" "(\<V>, \<C>) \<Turnstile>\<^sub>\<omega> \<omega>\<^sub>r" by (blast intro: static_eval_env.cases)+
 
   from `(\<V>, \<C>) \<Turnstile>\<^sub>\<rho> \<rho>` `\<rho> x\<^sub>s = Some \<lbrace>prim.Right x\<^sub>r', \<rho>\<^sub>r\<rbrace>`
-  have " | \<lbrace>prim.Right x\<^sub>r', \<rho>\<^sub>r\<rbrace> | \<in> \<V> x\<^sub>s" by (blast intro: accept_val_env.cases) then
+  have " | \<lbrace>prim.Right x\<^sub>r', \<rho>\<^sub>r\<rbrace> | \<in> \<V> x\<^sub>s" by (blast intro: static_eval_env.cases) then
   have "^prim.Right x\<^sub>r' \<in> \<V> x\<^sub>s" by simp
 
   from  `(\<V>, \<C>) \<Turnstile>\<^sub>e LET x = CASE x\<^sub>s LEFT x\<^sub>l |> e\<^sub>l RIGHT x\<^sub>r |> e\<^sub>r in e`
@@ -528,7 +528,7 @@ proof
     assume "(\<rho>(x\<^sub>r \<mapsto> \<omega>\<^sub>r)) x' = Some \<omega>'" "x' \<noteq> x\<^sub>r" then
     have "\<rho> x' = Some \<omega>'" by simp
     with `(\<V>, \<C>) \<Turnstile>\<^sub>\<rho> \<rho>` 
-    have "{|\<omega>'|} \<subseteq> \<V> x' \<and> (\<V>, \<C>) \<Turnstile>\<^sub>\<omega> \<omega>'" by (simp add: accept_val_env.simps)
+    have "{|\<omega>'|} \<subseteq> \<V> x' \<and> (\<V>, \<C>) \<Turnstile>\<^sub>\<omega> \<omega>'" by (simp add: static_eval_env.simps)
    
   }
   with `{|\<omega>\<^sub>r|} \<subseteq> \<V> x\<^sub>r` `(\<V>, \<C>) \<Turnstile>\<^sub>\<omega> \<omega>\<^sub>r`
@@ -549,7 +549,7 @@ proof
   have "(\<V>, \<C>) \<Turnstile>\<^sub>e LET x = CASE x\<^sub>s LEFT x\<^sub>l |> e\<^sub>l RIGHT x\<^sub>r |> e\<^sub>r in e" "(\<V>, \<C>) \<Turnstile>\<^sub>\<rho> \<rho>" by (blast intro: accept_state.cases)+
   
   from `(\<V>, \<C>) \<Turnstile>\<^sub>\<rho> \<rho>` `\<rho> x\<^sub>s = Some \<lbrace>prim.Right x\<^sub>r', \<rho>\<^sub>r\<rbrace>`
-  have " | \<lbrace>prim.Right x\<^sub>r', \<rho>\<^sub>r\<rbrace> | \<in> \<V> x\<^sub>s" by (blast intro: accept_val_env.cases) then
+  have " | \<lbrace>prim.Right x\<^sub>r', \<rho>\<^sub>r\<rbrace> | \<in> \<V> x\<^sub>s" by (blast intro: static_eval_env.cases) then
   have "^prim.Right x\<^sub>r' \<in> \<V> x\<^sub>s" by simp
 
   from `(\<V>, \<C>) \<Turnstile>\<^sub>e LET x = CASE x\<^sub>s LEFT x\<^sub>l |> e\<^sub>l RIGHT x\<^sub>r |> e\<^sub>r in e`
@@ -605,14 +605,14 @@ proof
   thm accept_state.simps
 
   from `(\<V>, \<C>) \<Turnstile>\<^sub>\<rho> \<rho>` `\<rho> x\<^sub>p = Some \<lbrace>prim.Pair x\<^sub>1 x\<^sub>2, \<rho>\<^sub>p\<rbrace>`
-  have "(\<V>, \<C>) \<Turnstile>\<^sub>\<omega> \<lbrace>prim.Pair x\<^sub>1 x\<^sub>2, \<rho>\<^sub>p\<rbrace>" by (blast intro: accept_val_env.cases) then
-  have "(\<V>, \<C>) \<Turnstile>\<^sub>\<rho> \<rho>\<^sub>p" by (blast intro: accept_value.cases)
+  have "(\<V>, \<C>) \<Turnstile>\<^sub>\<omega> \<lbrace>prim.Pair x\<^sub>1 x\<^sub>2, \<rho>\<^sub>p\<rbrace>" by (blast intro: static_eval_env.cases) then
+  have "(\<V>, \<C>) \<Turnstile>\<^sub>\<rho> \<rho>\<^sub>p" by (blast intro: static_eval_value.cases)
 
   from `(\<V>, \<C>) \<Turnstile>\<^sub>\<rho> \<rho>\<^sub>p` `\<rho>\<^sub>p x\<^sub>1 = Some \<omega>`
-  have "{|\<omega>|} \<subseteq> \<V> x\<^sub>1" "(\<V>, \<C>) \<Turnstile>\<^sub>\<omega> \<omega>" by (blast intro: accept_val_env.cases)+
+  have "{|\<omega>|} \<subseteq> \<V> x\<^sub>1" "(\<V>, \<C>) \<Turnstile>\<^sub>\<omega> \<omega>" by (blast intro: static_eval_env.cases)+
 
   from `(\<V>, \<C>) \<Turnstile>\<^sub>\<rho> \<rho>` `\<rho> x\<^sub>p = Some \<lbrace>prim.Pair x\<^sub>1 x\<^sub>2, \<rho>\<^sub>p\<rbrace>`
-  have " | \<lbrace>prim.Pair x\<^sub>1 x\<^sub>2, \<rho>\<^sub>p\<rbrace> | \<in> \<V> x\<^sub>p" by (blast intro: accept_val_env.cases) then
+  have " | \<lbrace>prim.Pair x\<^sub>1 x\<^sub>2, \<rho>\<^sub>p\<rbrace> | \<in> \<V> x\<^sub>p" by (blast intro: static_eval_env.cases) then
   have "^prim.Pair x\<^sub>1 x\<^sub>2 \<in> \<V> x\<^sub>p" by simp
 
   from  `(\<V>, \<C>) \<Turnstile>\<^sub>e LET x = FST x\<^sub>p in e`
@@ -632,7 +632,7 @@ proof
     assume "(\<rho>(x \<mapsto> \<omega>)) x' = Some \<omega>'" "x' \<noteq> x" then
     have "\<rho> x' = Some \<omega>'" by simp
     with `(\<V>, \<C>) \<Turnstile>\<^sub>\<rho> \<rho>` 
-    have "{|\<omega>'|} \<subseteq> \<V> x' \<and> (\<V>, \<C>) \<Turnstile>\<^sub>\<omega> \<omega>'" by (simp add: accept_val_env.simps)
+    have "{|\<omega>'|} \<subseteq> \<V> x' \<and> (\<V>, \<C>) \<Turnstile>\<^sub>\<omega> \<omega>'" by (simp add: static_eval_env.simps)
   }
   with `{|\<omega>|} \<subseteq> \<V> x` `(\<V>, \<C>) \<Turnstile>\<^sub>\<omega> \<omega>`
   show "\<forall>x' \<omega>'. (\<rho>(x \<mapsto> \<omega>)) x' = Some \<omega>' \<longrightarrow> {|\<omega>'|} \<subseteq> \<V> x' \<and> (\<V>, \<C>) \<Turnstile>\<^sub>\<omega> \<omega>'" by auto
@@ -668,14 +668,14 @@ proof
   have "(\<V>, \<C>) \<Turnstile>\<^sub>e LET x = SND x\<^sub>p in e" "(\<V>, \<C>) \<Turnstile>\<^sub>\<rho> \<rho>" by (simp add: accept_state.simps)+
 
   from `(\<V>, \<C>) \<Turnstile>\<^sub>\<rho> \<rho>` `\<rho> x\<^sub>p = Some \<lbrace>prim.Pair x\<^sub>1 x\<^sub>2, \<rho>\<^sub>p\<rbrace>`
-  have "(\<V>, \<C>) \<Turnstile>\<^sub>\<omega> \<lbrace>prim.Pair x\<^sub>1 x\<^sub>2, \<rho>\<^sub>p\<rbrace>" by (blast intro: accept_val_env.cases) then
-  have "(\<V>, \<C>) \<Turnstile>\<^sub>\<rho> \<rho>\<^sub>p" by (blast intro: accept_value.cases)
+  have "(\<V>, \<C>) \<Turnstile>\<^sub>\<omega> \<lbrace>prim.Pair x\<^sub>1 x\<^sub>2, \<rho>\<^sub>p\<rbrace>" by (blast intro: static_eval_env.cases) then
+  have "(\<V>, \<C>) \<Turnstile>\<^sub>\<rho> \<rho>\<^sub>p" by (blast intro: static_eval_value.cases)
 
   from `(\<V>, \<C>) \<Turnstile>\<^sub>\<rho> \<rho>\<^sub>p` `\<rho>\<^sub>p x\<^sub>2 = Some \<omega>`
-  have "{|\<omega>|} \<subseteq> \<V> x\<^sub>2" "(\<V>, \<C>) \<Turnstile>\<^sub>\<omega> \<omega>" by (blast intro: accept_val_env.cases)+
+  have "{|\<omega>|} \<subseteq> \<V> x\<^sub>2" "(\<V>, \<C>) \<Turnstile>\<^sub>\<omega> \<omega>" by (blast intro: static_eval_env.cases)+
 
   from `(\<V>, \<C>) \<Turnstile>\<^sub>\<rho> \<rho>` `\<rho> x\<^sub>p = Some \<lbrace>prim.Pair x\<^sub>1 x\<^sub>2, \<rho>\<^sub>p\<rbrace>`
-  have " | \<lbrace>prim.Pair x\<^sub>1 x\<^sub>2, \<rho>\<^sub>p\<rbrace> | \<in> \<V> x\<^sub>p" by (blast intro: accept_val_env.cases) then
+  have " | \<lbrace>prim.Pair x\<^sub>1 x\<^sub>2, \<rho>\<^sub>p\<rbrace> | \<in> \<V> x\<^sub>p" by (blast intro: static_eval_env.cases) then
   have "^prim.Pair x\<^sub>1 x\<^sub>2 \<in> \<V> x\<^sub>p" by simp
 
   from  `(\<V>, \<C>) \<Turnstile>\<^sub>e LET x = SND x\<^sub>p in e`
@@ -696,7 +696,7 @@ proof
     assume "(\<rho>(x \<mapsto> \<omega>)) x' = Some \<omega>'" "x' \<noteq> x" then
     have "\<rho> x' = Some \<omega>'" by simp
     with `(\<V>, \<C>) \<Turnstile>\<^sub>\<rho> \<rho>` 
-    have "{|\<omega>'|} \<subseteq> \<V> x' \<and> (\<V>, \<C>) \<Turnstile>\<^sub>\<omega> \<omega>'" by (simp add: accept_val_env.simps)
+    have "{|\<omega>'|} \<subseteq> \<V> x' \<and> (\<V>, \<C>) \<Turnstile>\<^sub>\<omega> \<omega>'" by (simp add: static_eval_env.simps)
   }
   with \<open>{|\<omega>|} \<subseteq> \<V> x\<close> \<open>(\<V>, \<C>) \<Turnstile>\<^sub>\<omega> \<omega>\<close> 
   show "\<forall>x' \<omega>'. (\<rho>(x \<mapsto> \<omega>)) x' = Some \<omega>' \<longrightarrow> {|\<omega>'|} \<subseteq> \<V> x' \<and> (\<V>, \<C>) \<Turnstile>\<^sub>\<omega> \<omega>'" by simp
@@ -733,16 +733,16 @@ proof
   have "(\<V>, \<C>) \<Turnstile>\<^sub>e LET x = APP f x\<^sub>a in e" "(\<V>, \<C>) \<Turnstile>\<^sub>\<rho> \<rho>" by (simp add: accept_state.simps)+
 
   from `(\<V>, \<C>) \<Turnstile>\<^sub>\<rho> \<rho>` and `\<rho> x\<^sub>a = Some \<omega>\<^sub>a`
-  have "{|\<omega>\<^sub>a|} \<subseteq> \<V> x\<^sub>a" "(\<V>, \<C>) \<Turnstile>\<^sub>\<omega> \<omega>\<^sub>a" by (blast intro: accept_val_env.cases)+
+  have "{|\<omega>\<^sub>a|} \<subseteq> \<V> x\<^sub>a" "(\<V>, \<C>) \<Turnstile>\<^sub>\<omega> \<omega>\<^sub>a" by (blast intro: static_eval_env.cases)+
 
   from `(\<V>, \<C>) \<Turnstile>\<^sub>\<rho> \<rho>` and `\<rho> f = Some \<lbrace>Abs f\<^sub>l x\<^sub>l e\<^sub>l, \<rho>\<^sub>l\<rbrace>`
-  have "{|\<lbrace>Abs f\<^sub>l x\<^sub>l e\<^sub>l, \<rho>\<^sub>l\<rbrace>|} \<subseteq> \<V> f" "(\<V>, \<C>) \<Turnstile>\<^sub>\<omega> \<lbrace>Abs f\<^sub>l x\<^sub>l e\<^sub>l, \<rho>\<^sub>l\<rbrace>" by (blast intro: accept_val_env.cases)+
+  have "{|\<lbrace>Abs f\<^sub>l x\<^sub>l e\<^sub>l, \<rho>\<^sub>l\<rbrace>|} \<subseteq> \<V> f" "(\<V>, \<C>) \<Turnstile>\<^sub>\<omega> \<lbrace>Abs f\<^sub>l x\<^sub>l e\<^sub>l, \<rho>\<^sub>l\<rbrace>" by (blast intro: static_eval_env.cases)+
 
   from `{|\<lbrace>Abs f\<^sub>l x\<^sub>l e\<^sub>l, \<rho>\<^sub>l\<rbrace>|} \<subseteq> \<V> f`
   have "^Abs f\<^sub>l x\<^sub>l e\<^sub>l \<in> \<V> f" by simp
 
   from `(\<V>, \<C>) \<Turnstile>\<^sub>\<omega> \<lbrace>Abs f\<^sub>l x\<^sub>l e\<^sub>l, \<rho>\<^sub>l\<rbrace>`
-  have "{|\<lbrace>Abs f\<^sub>l x\<^sub>l e\<^sub>l, \<rho>\<^sub>l\<rbrace>|} \<subseteq> \<V> f\<^sub>l" "(\<V>, \<C>) \<Turnstile>\<^sub>\<rho> \<rho>\<^sub>l" by (rule accept_value.cases; auto)+
+  have "{|\<lbrace>Abs f\<^sub>l x\<^sub>l e\<^sub>l, \<rho>\<^sub>l\<rbrace>|} \<subseteq> \<V> f\<^sub>l" "(\<V>, \<C>) \<Turnstile>\<^sub>\<rho> \<rho>\<^sub>l" by (rule static_eval_value.cases; auto)+
 
 
   with `(\<V>, \<C>) \<Turnstile>\<^sub>e LET x = APP f x\<^sub>a in e`
@@ -763,7 +763,7 @@ proof
     assume "(\<rho>\<^sub>l(f\<^sub>l \<mapsto> \<lbrace>Abs f\<^sub>l x\<^sub>l e\<^sub>l, \<rho>\<^sub>l\<rbrace>, x\<^sub>l \<mapsto> \<omega>\<^sub>a)) x' = Some \<omega>'" "x' \<noteq> x\<^sub>l" "x' \<noteq> f\<^sub>l" then
     have "\<rho>\<^sub>l x' = Some \<omega>'" by simp
     with `(\<V>, \<C>) \<Turnstile>\<^sub>\<rho> \<rho>\<^sub>l` 
-    have "{|\<omega>'|} \<subseteq> \<V> x' \<and> (\<V>, \<C>) \<Turnstile>\<^sub>\<omega> \<omega>'" by (simp add: accept_val_env.simps)
+    have "{|\<omega>'|} \<subseteq> \<V> x' \<and> (\<V>, \<C>) \<Turnstile>\<^sub>\<omega> \<omega>'" by (simp add: static_eval_env.simps)
   }
   with \<open>{|\<lbrace>Abs f\<^sub>l x\<^sub>l e\<^sub>l, \<rho>\<^sub>l\<rbrace>|} \<subseteq> \<V> f\<^sub>l\<close> \<open>(\<V>, \<C>) \<Turnstile>\<^sub>\<omega> \<lbrace>Abs f\<^sub>l x\<^sub>l e\<^sub>l, \<rho>\<^sub>l\<rbrace>\<close> \<open>(\<V>, \<C>) \<Turnstile>\<^sub>\<omega> \<omega>\<^sub>a\<close> \<open>{|\<omega>\<^sub>a|} \<subseteq> \<V> x\<^sub>l\<close>
   show "\<forall>x \<omega>. (\<rho>\<^sub>l(f\<^sub>l \<mapsto> \<lbrace>Abs f\<^sub>l x\<^sub>l e\<^sub>l, \<rho>\<^sub>l\<rbrace>, x\<^sub>l \<mapsto> \<omega>\<^sub>a)) x = Some \<omega> \<longrightarrow> {|\<omega>|} \<subseteq> \<V> x \<and> (\<V>, \<C>) \<Turnstile>\<^sub>\<omega> \<omega>" by auto
@@ -781,7 +781,7 @@ proof
   have "(\<V>, \<C>) \<Turnstile>\<^sub>e LET x = APP f x\<^sub>a in e"  "(\<V>, \<C>) \<Turnstile>\<^sub>\<rho> \<rho>" by (blast intro: accept_state.cases)+
 
   from `(\<V>, \<C>) \<Turnstile>\<^sub>\<rho> \<rho>` and `\<rho> f = Some \<lbrace>Abs f' x\<^sub>p e\<^sub>b, \<rho>'\<rbrace>`
-  have " {|\<lbrace>Abs f' x\<^sub>p e\<^sub>b, \<rho>'\<rbrace>|} \<subseteq> \<V> f" by (blast intro: accept_val_env.cases) then
+  have " {|\<lbrace>Abs f' x\<^sub>p e\<^sub>b, \<rho>'\<rbrace>|} \<subseteq> \<V> f" by (blast intro: static_eval_env.cases) then
   have " ^Abs f' x\<^sub>p e\<^sub>b \<in> \<V> f" by simp
 
   from `(\<V>, \<C>) \<Turnstile>\<^sub>e LET x = APP f x\<^sub>a in e`
@@ -896,13 +896,13 @@ lemma accept_preserved_under_seq_step_down: "
 proof
   
   assume "(\<V>, \<C>) \<Turnstile>\<^sub>\<E> \<E>" and "\<E> \<pi> = Some (\<langle>RESULT x; \<rho>; \<langle>x\<^sub>\<kappa>, e\<^sub>\<kappa>, \<rho>\<^sub>\<kappa>\<rangle> # \<kappa>\<rangle>)" then
-  have "(\<V>, \<C>) \<Turnstile>\<^sub>\<sigma> \<langle>RESULT x; \<rho>; \<langle>x\<^sub>\<kappa>, e\<^sub>\<kappa>, \<rho>\<^sub>\<kappa>\<rangle> # \<kappa>\<rangle>" by (simp add: accept_state_pool.simps)
+  have "(\<V>, \<C>) \<Turnstile>\<^sub>\<sigma> \<langle>RESULT x; \<rho>; \<langle>x\<^sub>\<kappa>, e\<^sub>\<kappa>, \<rho>\<^sub>\<kappa>\<rangle> # \<kappa>\<rangle>" by (simp add: static_eval_pool.simps)
   
   assume "\<langle>RESULT x; \<rho>; \<langle>x\<^sub>\<kappa>, e\<^sub>\<kappa>, \<rho>\<^sub>\<kappa>\<rangle> # \<kappa>\<rangle> \<hookrightarrow> \<sigma>'" with `(\<V>, \<C>) \<Turnstile>\<^sub>\<sigma> \<langle>RESULT x; \<rho>; \<langle>x\<^sub>\<kappa>, e\<^sub>\<kappa>, \<rho>\<^sub>\<kappa>\<rangle> # \<kappa>\<rangle>`
   have "(\<V>, \<C>) \<Turnstile>\<^sub>\<sigma> \<sigma>'" by (simp add: accept_state_preserved_under_step)
 
   from \<open>(\<V>, \<C>) \<Turnstile>\<^sub>\<E> \<E>\<close> \<open>(\<V>, \<C>) \<Turnstile>\<^sub>\<sigma> \<sigma>'\<close>
-  show "\<forall>\<pi>' \<sigma>. (\<E>(\<pi> ;; \<downharpoonleft>x\<^sub>\<kappa> \<mapsto> \<sigma>')) \<pi>' = Some \<sigma> \<longrightarrow> (\<V>, \<C>) \<Turnstile>\<^sub>\<sigma> \<sigma>" by (simp add: accept_state_pool.simps)
+  show "\<forall>\<pi>' \<sigma>. (\<E>(\<pi> ;; \<downharpoonleft>x\<^sub>\<kappa> \<mapsto> \<sigma>')) \<pi>' = Some \<sigma> \<longrightarrow> (\<V>, \<C>) \<Turnstile>\<^sub>\<sigma> \<sigma>" by (simp add: static_eval_pool.simps)
 
 qed
 
@@ -913,13 +913,13 @@ lemma accept_preserved_under_seq_step_up: "
 "
 proof
   assume "(\<V>, \<C>) \<Turnstile>\<^sub>\<E> \<E>" and "\<E> \<pi> = Some (\<langle>LET x = b in e; \<rho>; \<kappa>\<rangle>)" then
-  have "(\<V>, \<C>) \<Turnstile>\<^sub>\<sigma> \<langle>LET x = b in e; \<rho>; \<kappa>\<rangle>" by (simp add: accept_state_pool.simps)
+  have "(\<V>, \<C>) \<Turnstile>\<^sub>\<sigma> \<langle>LET x = b in e; \<rho>; \<kappa>\<rangle>" by (simp add: static_eval_pool.simps)
 
   assume "\<langle>LET x = b in e; \<rho>; \<kappa>\<rangle> \<hookrightarrow> \<sigma>'" with `(\<V>, \<C>) \<Turnstile>\<^sub>\<sigma> \<langle>LET x = b in e; \<rho>; \<kappa>\<rangle>`
   have "(\<V>, \<C>) \<Turnstile>\<^sub>\<sigma> \<sigma>'" by (simp add: accept_state_preserved_under_step)
 
   from \<open>(\<V>, \<C>) \<Turnstile>\<^sub>\<E> \<E>\<close> \<open>(\<V>, \<C>) \<Turnstile>\<^sub>\<sigma> \<sigma>'\<close>
-  show "\<forall>\<pi>' \<sigma>. (\<E>(\<pi> ;; \<upharpoonleft>x \<mapsto> \<sigma>')) \<pi>' = Some \<sigma> \<longrightarrow> (\<V>, \<C>) \<Turnstile>\<^sub>\<sigma> \<sigma>" by (simp add: accept_state_pool.simps)
+  show "\<forall>\<pi>' \<sigma>. (\<E>(\<pi> ;; \<upharpoonleft>x \<mapsto> \<sigma>')) \<pi>' = Some \<sigma> \<longrightarrow> (\<V>, \<C>) \<Turnstile>\<^sub>\<sigma> \<sigma>" by (simp add: static_eval_pool.simps)
 qed
 
 
@@ -929,13 +929,13 @@ lemma accept_preserved_under_seq_step: "
 "
 proof
   assume "(\<V>, \<C>) \<Turnstile>\<^sub>\<E> \<E>" and "\<E> \<pi> = Some (\<langle>LET x = b in e; \<rho>; \<kappa>\<rangle>)" then
-  have "(\<V>, \<C>) \<Turnstile>\<^sub>\<sigma> \<langle>LET x = b in e; \<rho>; \<kappa>\<rangle>" by (simp add: accept_state_pool.simps)
+  have "(\<V>, \<C>) \<Turnstile>\<^sub>\<sigma> \<langle>LET x = b in e; \<rho>; \<kappa>\<rangle>" by (simp add: static_eval_pool.simps)
 
   assume "\<langle>LET x = b in e; \<rho>; \<kappa>\<rangle> \<hookrightarrow> \<sigma>'" with `(\<V>, \<C>) \<Turnstile>\<^sub>\<sigma> \<langle>LET x = b in e; \<rho>; \<kappa>\<rangle>`
   have "(\<V>, \<C>) \<Turnstile>\<^sub>\<sigma> \<sigma>'" by (simp add: accept_state_preserved_under_step)
 
   from \<open>(\<V>, \<C>) \<Turnstile>\<^sub>\<E> \<E>\<close> \<open>(\<V>, \<C>) \<Turnstile>\<^sub>\<sigma> \<sigma>'\<close>
-  show "\<forall>\<pi>' \<sigma>. (\<E>(\<pi> ;; `x \<mapsto> \<sigma>')) \<pi>' = Some \<sigma> \<longrightarrow> (\<V>, \<C>) \<Turnstile>\<^sub>\<sigma> \<sigma>" by (simp add: accept_state_pool.simps)
+  show "\<forall>\<pi>' \<sigma>. (\<E>(\<pi> ;; `x \<mapsto> \<sigma>')) \<pi>' = Some \<sigma> \<longrightarrow> (\<V>, \<C>) \<Turnstile>\<^sub>\<sigma> \<sigma>" by (simp add: static_eval_pool.simps)
 qed
 
 lemma accept_pool_to_exp_let: "
@@ -945,7 +945,7 @@ lemma accept_pool_to_exp_let: "
 "
 proof -
  assume "(\<V>, \<C>) \<Turnstile>\<^sub>\<E> \<E>" and "\<E> \<pi> = Some (\<langle>LET x = b in e; \<rho>; \<kappa>\<rangle>)" then
- have "(\<V>, \<C>) \<Turnstile>\<^sub>\<sigma> \<langle>LET x = b in e; \<rho>; \<kappa>\<rangle>" by (simp add: accept_state_pool.simps) then
+ have "(\<V>, \<C>) \<Turnstile>\<^sub>\<sigma> \<langle>LET x = b in e; \<rho>; \<kappa>\<rangle>" by (simp add: static_eval_pool.simps) then
  show "(\<V>, \<C>) \<Turnstile>\<^sub>e e " by (blast intro: accept_state_to_exp_let)
 qed
 
@@ -964,19 +964,19 @@ proof -
   and "\<rho>\<^sub>s\<^sub>e x\<^sub>s\<^sub>c = Some \<lbrace>Ch \<pi>\<^sub>c x\<^sub>c\<rbrace>"
 
   from `(\<V>, \<C>) \<Turnstile>\<^sub>\<E> \<E>` and `\<E> \<pi>\<^sub>s = Some (\<langle>LET x\<^sub>s = SYNC x\<^sub>s\<^sub>e in e\<^sub>s; \<rho>\<^sub>s; \<kappa>\<^sub>s\<rangle>)`
-  have "(\<V>, \<C>) \<Turnstile>\<^sub>\<sigma> \<langle>LET x\<^sub>s = SYNC x\<^sub>s\<^sub>e in e\<^sub>s; \<rho>\<^sub>s; \<kappa>\<^sub>s\<rangle>" by (simp add: accept_state_pool.simps) then
+  have "(\<V>, \<C>) \<Turnstile>\<^sub>\<sigma> \<langle>LET x\<^sub>s = SYNC x\<^sub>s\<^sub>e in e\<^sub>s; \<rho>\<^sub>s; \<kappa>\<^sub>s\<rangle>" by (simp add: static_eval_pool.simps) then
   have "(\<V>, \<C>) \<Turnstile>\<^sub>e LET x\<^sub>s = SYNC x\<^sub>s\<^sub>e in e\<^sub>s" "(\<V>, \<C>) \<Turnstile>\<^sub>\<rho> \<rho>\<^sub>s" by (simp add: accept_state.simps)+
 
   from `(\<V>, \<C>) \<Turnstile>\<^sub>\<rho> \<rho>\<^sub>s` and `\<rho>\<^sub>s x\<^sub>s\<^sub>e = Some \<lbrace>Send_Evt x\<^sub>s\<^sub>c x\<^sub>m, \<rho>\<^sub>s\<^sub>e\<rbrace>`
-  have "{|\<lbrace>Send_Evt x\<^sub>s\<^sub>c x\<^sub>m, \<rho>\<^sub>s\<^sub>e\<rbrace>|} \<subseteq> \<V> x\<^sub>s\<^sub>e" and "(\<V>, \<C>) \<Turnstile>\<^sub>\<omega> \<lbrace>Send_Evt x\<^sub>s\<^sub>c x\<^sub>m, \<rho>\<^sub>s\<^sub>e\<rbrace>" by (blast intro: accept_val_env.cases)+
+  have "{|\<lbrace>Send_Evt x\<^sub>s\<^sub>c x\<^sub>m, \<rho>\<^sub>s\<^sub>e\<rbrace>|} \<subseteq> \<V> x\<^sub>s\<^sub>e" and "(\<V>, \<C>) \<Turnstile>\<^sub>\<omega> \<lbrace>Send_Evt x\<^sub>s\<^sub>c x\<^sub>m, \<rho>\<^sub>s\<^sub>e\<rbrace>" by (blast intro: static_eval_env.cases)+
 
   from `{|\<lbrace>Send_Evt x\<^sub>s\<^sub>c x\<^sub>m, \<rho>\<^sub>s\<^sub>e\<rbrace>|} \<subseteq> \<V> x\<^sub>s\<^sub>e`
   have "^Send_Evt x\<^sub>s\<^sub>c x\<^sub>m \<in> \<V> x\<^sub>s\<^sub>e" by simp
 
   from `(\<V>, \<C>) \<Turnstile>\<^sub>\<omega> \<lbrace>Send_Evt x\<^sub>s\<^sub>c x\<^sub>m, \<rho>\<^sub>s\<^sub>e\<rbrace>`
-  have "(\<V>, \<C>) \<Turnstile>\<^sub>\<rho> \<rho>\<^sub>s\<^sub>e" by (blast intro: accept_value.cases)
+  have "(\<V>, \<C>) \<Turnstile>\<^sub>\<rho> \<rho>\<^sub>s\<^sub>e" by (blast intro: static_eval_value.cases)
   with `\<rho>\<^sub>s\<^sub>e x\<^sub>s\<^sub>c = Some \<lbrace>Ch \<pi>\<^sub>c x\<^sub>c\<rbrace>`
-  have "{|\<lbrace>Ch \<pi>\<^sub>c x\<^sub>c\<rbrace>|} \<subseteq> \<V> x\<^sub>s\<^sub>c" by (blast intro: accept_val_env.cases) then
+  have "{|\<lbrace>Ch \<pi>\<^sub>c x\<^sub>c\<rbrace>|} \<subseteq> \<V> x\<^sub>s\<^sub>c" by (blast intro: static_eval_env.cases) then
   have "{^Chan x\<^sub>c} \<subseteq> \<V> x\<^sub>s\<^sub>c" by simp then
   have "^Chan x\<^sub>c \<in> \<V> x\<^sub>s\<^sub>c" by auto
   
@@ -1005,13 +1005,13 @@ proof -
   and "\<rho>\<^sub>s\<^sub>e x\<^sub>m = Some \<omega>\<^sub>m"
 
   from `(\<V>, \<C>) \<Turnstile>\<^sub>\<E> \<E>` and `\<E> \<pi>\<^sub>s = Some (\<langle>LET x\<^sub>s = SYNC x\<^sub>s\<^sub>e in e\<^sub>s; \<rho>\<^sub>s; \<kappa>\<^sub>s\<rangle>)`
-  have "(\<V>, \<C>) \<Turnstile>\<^sub>\<sigma> \<langle>LET x\<^sub>s = SYNC x\<^sub>s\<^sub>e in e\<^sub>s; \<rho>\<^sub>s; \<kappa>\<^sub>s\<rangle>" by (simp add: accept_state_pool.simps) then
+  have "(\<V>, \<C>) \<Turnstile>\<^sub>\<sigma> \<langle>LET x\<^sub>s = SYNC x\<^sub>s\<^sub>e in e\<^sub>s; \<rho>\<^sub>s; \<kappa>\<^sub>s\<rangle>" by (simp add: static_eval_pool.simps) then
   have "(\<V>, \<C>) \<Turnstile>\<^sub>\<rho> \<rho>\<^sub>s" by (simp add: accept_state.simps)
   with `\<rho>\<^sub>s x\<^sub>s\<^sub>e = Some \<lbrace>Send_Evt x\<^sub>s\<^sub>c x\<^sub>m, \<rho>\<^sub>s\<^sub>e\<rbrace>`
-  have "(\<V>, \<C>) \<Turnstile>\<^sub>\<omega> \<lbrace>Send_Evt x\<^sub>s\<^sub>c x\<^sub>m, \<rho>\<^sub>s\<^sub>e\<rbrace>" by (blast intro: accept_val_env.cases) then
-  have "(\<V>, \<C>) \<Turnstile>\<^sub>\<rho> \<rho>\<^sub>s\<^sub>e" by (blast intro: accept_value.cases)
+  have "(\<V>, \<C>) \<Turnstile>\<^sub>\<omega> \<lbrace>Send_Evt x\<^sub>s\<^sub>c x\<^sub>m, \<rho>\<^sub>s\<^sub>e\<rbrace>" by (blast intro: static_eval_env.cases) then
+  have "(\<V>, \<C>) \<Turnstile>\<^sub>\<rho> \<rho>\<^sub>s\<^sub>e" by (blast intro: static_eval_value.cases)
   with `\<rho>\<^sub>s\<^sub>e x\<^sub>m = Some \<omega>\<^sub>m`
-  show "{|\<omega>\<^sub>m|} \<subseteq> \<V> x\<^sub>m \<and> (\<V>, \<C>) \<Turnstile>\<^sub>\<omega> \<omega>\<^sub>m" by (blast intro: accept_val_env.cases)
+  show "{|\<omega>\<^sub>m|} \<subseteq> \<V> x\<^sub>m \<and> (\<V>, \<C>) \<Turnstile>\<^sub>\<omega> \<omega>\<^sub>m" by (blast intro: static_eval_env.cases)
 qed
 
 lemma accept_pool_to_env_let_sync_send: "
@@ -1028,7 +1028,7 @@ proof
   and "\<rho>\<^sub>s x\<^sub>s\<^sub>e = Some \<lbrace>Send_Evt x\<^sub>s\<^sub>c x\<^sub>m, \<rho>\<^sub>s\<^sub>e\<rbrace>"
 
   from `(\<V>, \<C>) \<Turnstile>\<^sub>\<E> \<E>` and `\<E> \<pi>\<^sub>s = Some (\<langle>LET x\<^sub>s = SYNC x\<^sub>s\<^sub>e in e\<^sub>s; \<rho>\<^sub>s; \<kappa>\<^sub>s\<rangle>)`
-  have "(\<V>, \<C>) \<Turnstile>\<^sub>\<sigma> \<langle>LET x\<^sub>s = SYNC x\<^sub>s\<^sub>e in e\<^sub>s; \<rho>\<^sub>s; \<kappa>\<^sub>s\<rangle>" by (simp add: accept_state_pool.simps) then
+  have "(\<V>, \<C>) \<Turnstile>\<^sub>\<sigma> \<langle>LET x\<^sub>s = SYNC x\<^sub>s\<^sub>e in e\<^sub>s; \<rho>\<^sub>s; \<kappa>\<^sub>s\<rangle>" by (simp add: static_eval_pool.simps) then
   have "(\<V>, \<C>) \<Turnstile>\<^sub>\<rho> \<rho>\<^sub>s" by (simp add: accept_state.simps)+
 
   have "{^\<lparr>\<rparr>} \<subseteq> \<V> x\<^sub>s"
@@ -1048,7 +1048,7 @@ proof
     assume "(\<rho>\<^sub>s(x\<^sub>s \<mapsto> \<lbrace>\<rbrace>)) x' = Some \<omega>'" "x' \<noteq> x\<^sub>s" then
     have "\<rho>\<^sub>s x' = Some \<omega>'" by simp
     with `(\<V>, \<C>) \<Turnstile>\<^sub>\<rho> \<rho>\<^sub>s` 
-    have "{|\<omega>'|} \<subseteq> \<V> x' \<and> (\<V>, \<C>) \<Turnstile>\<^sub>\<omega> \<omega>'" by (simp add: accept_val_env.simps)
+    have "{|\<omega>'|} \<subseteq> \<V> x' \<and> (\<V>, \<C>) \<Turnstile>\<^sub>\<omega> \<omega>'" by (simp add: static_eval_env.simps)
   }
   with \<open>{^\<lparr>\<rparr>} \<subseteq> \<V> x\<^sub>s\<close> \<open>(\<V>, \<C>) \<Turnstile>\<^sub>\<omega> \<lbrace>\<rbrace>\<close> 
   show "\<forall>x \<omega>. (\<rho>\<^sub>s(x\<^sub>s \<mapsto> \<lbrace>\<rbrace>)) x = Some \<omega> \<longrightarrow> {|\<omega>|} \<subseteq> \<V> x \<and> (\<V>, \<C>) \<Turnstile>\<^sub>\<omega> \<omega>" by simp
@@ -1069,19 +1069,19 @@ proof -
   and "\<rho>\<^sub>r\<^sub>e x\<^sub>r\<^sub>c = Some \<lbrace>Ch \<pi>\<^sub>c x\<^sub>c\<rbrace>"
 
   from `(\<V>, \<C>) \<Turnstile>\<^sub>\<E> \<E>` and `\<E> \<pi>\<^sub>r = Some (\<langle>LET x\<^sub>r = SYNC x\<^sub>r\<^sub>e in e\<^sub>r; \<rho>\<^sub>r; \<kappa>\<^sub>r\<rangle>)`
-  have "(\<V>, \<C>) \<Turnstile>\<^sub>\<sigma> \<langle>LET x\<^sub>r = SYNC x\<^sub>r\<^sub>e in e\<^sub>r; \<rho>\<^sub>r; \<kappa>\<^sub>r\<rangle>" by (simp add: accept_state_pool.simps) then
+  have "(\<V>, \<C>) \<Turnstile>\<^sub>\<sigma> \<langle>LET x\<^sub>r = SYNC x\<^sub>r\<^sub>e in e\<^sub>r; \<rho>\<^sub>r; \<kappa>\<^sub>r\<rangle>" by (simp add: static_eval_pool.simps) then
   have "(\<V>, \<C>) \<Turnstile>\<^sub>e LET x\<^sub>r = SYNC x\<^sub>r\<^sub>e in e\<^sub>r" "(\<V>, \<C>) \<Turnstile>\<^sub>\<rho> \<rho>\<^sub>r" by (simp add: accept_state.simps)+
 
   from `(\<V>, \<C>) \<Turnstile>\<^sub>\<rho> \<rho>\<^sub>r` and `\<rho>\<^sub>r x\<^sub>r\<^sub>e = Some \<lbrace>Recv_Evt x\<^sub>r\<^sub>c, \<rho>\<^sub>r\<^sub>e\<rbrace>`
-  have "{|\<lbrace>Recv_Evt x\<^sub>r\<^sub>c, \<rho>\<^sub>r\<^sub>e\<rbrace>|} \<subseteq> \<V> x\<^sub>r\<^sub>e" and "(\<V>, \<C>) \<Turnstile>\<^sub>\<omega> \<lbrace>Recv_Evt x\<^sub>r\<^sub>c, \<rho>\<^sub>r\<^sub>e\<rbrace>" by (blast intro: accept_val_env.cases)+
+  have "{|\<lbrace>Recv_Evt x\<^sub>r\<^sub>c, \<rho>\<^sub>r\<^sub>e\<rbrace>|} \<subseteq> \<V> x\<^sub>r\<^sub>e" and "(\<V>, \<C>) \<Turnstile>\<^sub>\<omega> \<lbrace>Recv_Evt x\<^sub>r\<^sub>c, \<rho>\<^sub>r\<^sub>e\<rbrace>" by (blast intro: static_eval_env.cases)+
 
   from `{|\<lbrace>Recv_Evt x\<^sub>r\<^sub>c, \<rho>\<^sub>r\<^sub>e\<rbrace>|} \<subseteq> \<V> x\<^sub>r\<^sub>e`
   have "^Recv_Evt x\<^sub>r\<^sub>c \<in> \<V> x\<^sub>r\<^sub>e" by simp
 
   from `(\<V>, \<C>) \<Turnstile>\<^sub>\<omega> \<lbrace>Recv_Evt x\<^sub>r\<^sub>c, \<rho>\<^sub>r\<^sub>e\<rbrace>`
-  have "(\<V>, \<C>) \<Turnstile>\<^sub>\<rho> \<rho>\<^sub>r\<^sub>e" by (blast intro: accept_value.cases)
+  have "(\<V>, \<C>) \<Turnstile>\<^sub>\<rho> \<rho>\<^sub>r\<^sub>e" by (blast intro: static_eval_value.cases)
   with `\<rho>\<^sub>r\<^sub>e x\<^sub>r\<^sub>c = Some \<lbrace>Ch \<pi>\<^sub>c x\<^sub>c\<rbrace>`
-  have "{|\<lbrace>Ch \<pi>\<^sub>c x\<^sub>c\<rbrace>|} \<subseteq> \<V> x\<^sub>r\<^sub>c" by (blast intro: accept_val_env.cases) then
+  have "{|\<lbrace>Ch \<pi>\<^sub>c x\<^sub>c\<rbrace>|} \<subseteq> \<V> x\<^sub>r\<^sub>c" by (blast intro: static_eval_env.cases) then
   have "{^Chan x\<^sub>c} \<subseteq> \<V> x\<^sub>r\<^sub>c" by simp then
   have "^Chan x\<^sub>c \<in> \<V> x\<^sub>r\<^sub>c" by auto
   
@@ -1103,7 +1103,7 @@ lemma accept_pool_to_stack_let: "
 "
 proof -
   assume "(\<V>, \<C>) \<Turnstile>\<^sub>\<E> \<E>" and "\<E> \<pi> = Some (\<langle>LET x = b in e; \<rho>; \<kappa>\<rangle>)" then
-  have "(\<V>, \<C>) \<Turnstile>\<^sub>\<sigma> \<langle>LET x = b in e; \<rho>; \<kappa>\<rangle>" by (simp add: accept_state_pool.simps) then
+  have "(\<V>, \<C>) \<Turnstile>\<^sub>\<sigma> \<langle>LET x = b in e; \<rho>; \<kappa>\<rangle>" by (simp add: static_eval_pool.simps) then
   show "(\<V>, \<C>) \<Turnstile>\<^sub>\<kappa> \<V> (\<lfloor>e\<rfloor>) \<Rrightarrow> \<kappa>" by (simp add: accept_state_to_stack_let)
 qed
 
@@ -1131,7 +1131,7 @@ proof
   and "\<rho>\<^sub>r\<^sub>e x\<^sub>r\<^sub>c = Some \<lbrace>c\<rbrace>"
 
   from `(\<V>, \<C>) \<Turnstile>\<^sub>\<E> \<E>` and `\<E> \<pi>\<^sub>r = Some (\<langle>LET x\<^sub>r = SYNC x\<^sub>r\<^sub>e in e\<^sub>r; \<rho>\<^sub>r; \<kappa>\<^sub>r\<rangle>)`
-  have "(\<V>, \<C>) \<Turnstile>\<^sub>\<sigma> \<langle>LET x\<^sub>r = SYNC x\<^sub>r\<^sub>e in e\<^sub>r; \<rho>\<^sub>r; \<kappa>\<^sub>r\<rangle>" by (simp add: accept_state_pool.simps) then
+  have "(\<V>, \<C>) \<Turnstile>\<^sub>\<sigma> \<langle>LET x\<^sub>r = SYNC x\<^sub>r\<^sub>e in e\<^sub>r; \<rho>\<^sub>r; \<kappa>\<^sub>r\<rangle>" by (simp add: static_eval_pool.simps) then
   have "(\<V>, \<C>) \<Turnstile>\<^sub>\<rho> \<rho>\<^sub>r" by (simp add: accept_state.simps)+
 
 
@@ -1163,14 +1163,14 @@ proof
   have "{|\<omega>\<^sub>m|} \<subseteq> \<V> x\<^sub>r" by blast
 
   from `(\<V>, \<C>) \<Turnstile>\<^sub>\<E> \<E>` and `\<E> \<pi>\<^sub>s = Some (\<langle>LET x\<^sub>s = SYNC x\<^sub>s\<^sub>e in e\<^sub>s; \<rho>\<^sub>s; \<kappa>\<^sub>s\<rangle>)`
-  have "(\<V>, \<C>) \<Turnstile>\<^sub>\<sigma> \<langle>LET x\<^sub>s = SYNC x\<^sub>s\<^sub>e in e\<^sub>s; \<rho>\<^sub>s; \<kappa>\<^sub>s\<rangle>" by (simp add: accept_state_pool.simps) then
+  have "(\<V>, \<C>) \<Turnstile>\<^sub>\<sigma> \<langle>LET x\<^sub>s = SYNC x\<^sub>s\<^sub>e in e\<^sub>s; \<rho>\<^sub>s; \<kappa>\<^sub>s\<rangle>" by (simp add: static_eval_pool.simps) then
   have "(\<V>, \<C>) \<Turnstile>\<^sub>\<rho> \<rho>\<^sub>s" by (simp add: accept_state.simps)+
   {
     fix x' \<omega>'
     assume "(\<rho>\<^sub>r(x\<^sub>r \<mapsto> \<omega>\<^sub>m)) x' = Some \<omega>'" "x' \<noteq> x\<^sub>r" then
     have "\<rho>\<^sub>r x' = Some \<omega>'" by simp
     with `(\<V>, \<C>) \<Turnstile>\<^sub>\<rho> \<rho>\<^sub>r` 
-    have "{|\<omega>'|} \<subseteq> \<V> x' \<and> (\<V>, \<C>) \<Turnstile>\<^sub>\<omega> \<omega>'" by (simp add: accept_val_env.simps)
+    have "{|\<omega>'|} \<subseteq> \<V> x' \<and> (\<V>, \<C>) \<Turnstile>\<^sub>\<omega> \<omega>'" by (simp add: static_eval_env.simps)
   }
   with `{|\<omega>\<^sub>m|} \<subseteq> \<V> x\<^sub>r` and `(\<V>, \<C>) \<Turnstile>\<^sub>\<omega> \<omega>\<^sub>m`
   show "\<forall>x \<omega>. (\<rho>\<^sub>r(x\<^sub>r \<mapsto> \<omega>\<^sub>m)) x = Some \<omega> \<longrightarrow> {|\<omega>|} \<subseteq> \<V> x \<and> (\<V>, \<C>) \<Turnstile>\<^sub>\<omega> \<omega>" by auto
@@ -1235,7 +1235,7 @@ proof
     and "(\<E>(\<pi>\<^sub>s ;; `x\<^sub>s \<mapsto> \<langle>e\<^sub>s;\<rho>\<^sub>s(x\<^sub>s \<mapsto> \<lbrace>\<rbrace>);\<kappa>\<^sub>s\<rangle>, \<pi>\<^sub>r ;; `x\<^sub>r \<mapsto> \<langle>e\<^sub>r;\<rho>\<^sub>r(x\<^sub>r \<mapsto> \<omega>\<^sub>m);\<kappa>\<^sub>r\<rangle>)) \<pi> = Some \<sigma>" then
     have "\<E> \<pi> = Some \<sigma>" by simp
     with \<open>(\<V>, \<C>) \<Turnstile>\<^sub>\<E> \<E>\<close>
-    have "(\<V>, \<C>) \<Turnstile>\<^sub>\<sigma> \<sigma>" by (blast intro: accept_state_pool.cases)
+    have "(\<V>, \<C>) \<Turnstile>\<^sub>\<sigma> \<sigma>" by (blast intro: static_eval_pool.cases)
   } with `(\<V>, \<C>) \<Turnstile>\<^sub>\<sigma> \<langle>e\<^sub>r;\<rho>\<^sub>r (x\<^sub>r \<mapsto> \<omega>\<^sub>m);\<kappa>\<^sub>r\<rangle>` `(\<V>, \<C>) \<Turnstile>\<^sub>\<sigma> \<langle>e\<^sub>s;\<rho>\<^sub>s (x\<^sub>s \<mapsto> \<lbrace>\<rbrace>);\<kappa>\<^sub>s\<rangle>`
   show "\<forall>\<pi> \<sigma>. (\<E>(\<pi>\<^sub>s ;; `x\<^sub>s \<mapsto> \<langle>e\<^sub>s;\<rho>\<^sub>s(x\<^sub>s \<mapsto> \<lbrace>\<rbrace>);\<kappa>\<^sub>s\<rangle>, \<pi>\<^sub>r ;; `x\<^sub>r \<mapsto> \<langle>e\<^sub>r;\<rho>\<^sub>r(x\<^sub>r \<mapsto> \<omega>\<^sub>m);\<kappa>\<^sub>r\<rangle>)) \<pi> = Some \<sigma> \<longrightarrow> (\<V>, \<C>) \<Turnstile>\<^sub>\<sigma> \<sigma>" by simp
 
@@ -1249,9 +1249,9 @@ lemma accept_pool_to_env_let_chan: "
 "
 proof
   assume "(\<V>, \<C>) \<Turnstile>\<^sub>\<E> \<E>" and "\<E> \<pi> = Some (\<langle>LET x = CHAN \<lparr>\<rparr> in e; \<rho>; \<kappa>\<rangle>)" then
-  have "(\<V>, \<C>) \<Turnstile>\<^sub>\<sigma> \<langle>LET x = CHAN \<lparr>\<rparr> in e; \<rho>; \<kappa>\<rangle>" by (blast intro: accept_state_pool.cases) then
+  have "(\<V>, \<C>) \<Turnstile>\<^sub>\<sigma> \<langle>LET x = CHAN \<lparr>\<rparr> in e; \<rho>; \<kappa>\<rangle>" by (blast intro: static_eval_pool.cases) then
   have "(\<V>, \<C>) \<Turnstile>\<^sub>e LET x = CHAN \<lparr>\<rparr> in e" by (blast intro: accept_state.cases) then
-  have "{^Chan x} \<subseteq> \<V> x"  by (blast intro: accept_exp.cases)
+  have "{^Chan x} \<subseteq> \<V> x"  by (blast intro: static_eval.cases)
   have "(\<V>, \<C>) \<Turnstile>\<^sub>\<omega> \<lbrace>Ch \<pi> x\<rbrace>" by (simp add: Chan)
 
   from `(\<V>, \<C>) \<Turnstile>\<^sub>\<sigma> \<langle>LET x = CHAN \<lparr>\<rparr> in e; \<rho>; \<kappa>\<rangle>` 
@@ -1260,7 +1260,7 @@ proof
     fix x' \<omega>'
     assume "(\<rho>(x \<mapsto> \<lbrace>Ch \<pi> x\<rbrace>)) x' = Some \<omega>'" and "x \<noteq> x'"then
     have "\<rho> x' = Some \<omega>'" by simp with `(\<V>, \<C>) \<Turnstile>\<^sub>\<rho> \<rho>`
-    have "{|\<omega>'|} \<subseteq> \<V> x' \<and> (\<V>, \<C>) \<Turnstile>\<^sub>\<omega> \<omega>'" by (simp add: accept_val_env.simps)
+    have "{|\<omega>'|} \<subseteq> \<V> x' \<and> (\<V>, \<C>) \<Turnstile>\<^sub>\<omega> \<omega>'" by (simp add: static_eval_env.simps)
   } with `{^Chan x} \<subseteq> \<V> x` and `(\<V>, \<C>) \<Turnstile>\<^sub>\<omega> \<lbrace>Ch \<pi> x\<rbrace>`
   show "\<forall>x' \<omega>'. (\<rho>(x \<mapsto> \<lbrace>Ch \<pi> x\<rbrace>)) x' = Some \<omega>' \<longrightarrow> {|\<omega>'|} \<subseteq> \<V> x' \<and> (\<V>, \<C>) \<Turnstile>\<^sub>\<omega> \<omega>'" by simp
 qed
@@ -1288,7 +1288,7 @@ proof
     assume "(\<E>(\<pi> ;; `x \<mapsto> \<langle>e;\<rho>(x \<mapsto> \<lbrace>Ch \<pi> x\<rbrace>);\<kappa>\<rangle>)) \<pi>' = Some \<sigma>'" 
     and "\<pi>' \<noteq> \<pi> ;; `x" then
     have "\<E> \<pi>' = Some \<sigma>'" by simp with `(\<V>, \<C>) \<Turnstile>\<^sub>\<E> \<E>`
-    have "(\<V>, \<C>) \<Turnstile>\<^sub>\<sigma> \<sigma>'" by (simp add: accept_state_pool.simps)
+    have "(\<V>, \<C>) \<Turnstile>\<^sub>\<sigma> \<sigma>'" by (simp add: static_eval_pool.simps)
   } with `(\<V>, \<C>) \<Turnstile>\<^sub>\<sigma> \<langle>e;\<rho>(x \<mapsto> \<lbrace>Ch \<pi> x\<rbrace>);\<kappa>\<rangle>`
   show "\<forall>\<pi>' \<sigma>'. (\<E>(\<pi> ;; `x \<mapsto> \<langle>e;\<rho>(x \<mapsto> \<lbrace>Ch \<pi> x\<rbrace>);\<kappa>\<rangle>)) \<pi>' = Some \<sigma>' \<longrightarrow> (\<V>, \<C>) \<Turnstile>\<^sub>\<sigma> \<sigma>'" by simp
 qed
@@ -1301,9 +1301,9 @@ lemma accept_pool_to_env_let_spawn: "
 proof
 
   assume "(\<V>, \<C>) \<Turnstile>\<^sub>\<E> \<E>" and "\<E> \<pi> = Some (\<langle>LET x = SPAWN e\<^sub>c in e; \<rho>; \<kappa>\<rangle>)" then
-  have "(\<V>, \<C>) \<Turnstile>\<^sub>\<sigma> \<langle>LET x = SPAWN e\<^sub>c in e; \<rho>; \<kappa>\<rangle>" by (simp add: accept_state_pool.simps) then
+  have "(\<V>, \<C>) \<Turnstile>\<^sub>\<sigma> \<langle>LET x = SPAWN e\<^sub>c in e; \<rho>; \<kappa>\<rangle>" by (simp add: static_eval_pool.simps) then
   have "(\<V>, \<C>) \<Turnstile>\<^sub>e LET x = SPAWN e\<^sub>c in e" by (blast intro: accept_state.cases) then
-  have "{^\<lparr>\<rparr>} \<subseteq> \<V> x"  by (blast intro: accept_exp.cases) then
+  have "{^\<lparr>\<rparr>} \<subseteq> \<V> x"  by (blast intro: static_eval.cases) then
   have "(\<V>, \<C>) \<Turnstile>\<^sub>\<omega> \<lbrace>\<rbrace>" by (simp add: Unit)
 
   from `(\<V>, \<C>) \<Turnstile>\<^sub>\<sigma> \<langle>LET x = SPAWN e\<^sub>c in e; \<rho>; \<kappa>\<rangle>` 
@@ -1313,7 +1313,7 @@ proof
     fix x' \<omega>'
     assume "(\<rho>(x \<mapsto> \<lbrace>\<rbrace>)) x' = Some \<omega>'" and "x \<noteq> x'" then
     have "\<rho> x' = Some \<omega>'" by simp with `(\<V>, \<C>) \<Turnstile>\<^sub>\<rho> \<rho>`
-    have "{|\<omega>'|} \<subseteq> \<V> x' \<and> (\<V>, \<C>) \<Turnstile>\<^sub>\<omega> \<omega>'" by (blast intro: accept_val_env.cases)
+    have "{|\<omega>'|} \<subseteq> \<V> x' \<and> (\<V>, \<C>) \<Turnstile>\<^sub>\<omega> \<omega>'" by (blast intro: static_eval_env.cases)
   } with `{^\<lparr>\<rparr>} \<subseteq> \<V> x` and `(\<V>, \<C>) \<Turnstile>\<^sub>\<omega> \<lbrace>\<rbrace>`
   show "\<forall>x' \<omega>'. (\<rho>(x \<mapsto> \<lbrace>\<rbrace>)) x' = Some \<omega>' \<longrightarrow> {|\<omega>'|} \<subseteq> \<V> x' \<and> (\<V>, \<C>) \<Turnstile>\<^sub>\<omega> \<omega>'" by simp
 qed
@@ -1340,13 +1340,13 @@ proof
   have "(\<V>, \<C>) \<Turnstile>\<^sub>\<sigma> \<langle>e;\<rho>(x \<mapsto> \<lbrace>\<rbrace>);\<kappa>\<rangle>" by (simp add: accept_state.intros)
 
   from `(\<V>, \<C>) \<Turnstile>\<^sub>\<E> \<E>` and `\<E> \<pi> = Some (\<langle>LET x = SPAWN e\<^sub>c in e; \<rho>; \<kappa>\<rangle>)`
-  have "(\<V>, \<C>) \<Turnstile>\<^sub>\<sigma> \<langle>LET x = SPAWN e\<^sub>c in e; \<rho>; \<kappa>\<rangle>" by (simp add: accept_state_pool.simps) then
+  have "(\<V>, \<C>) \<Turnstile>\<^sub>\<sigma> \<langle>LET x = SPAWN e\<^sub>c in e; \<rho>; \<kappa>\<rangle>" by (simp add: static_eval_pool.simps) then
   have "(\<V>, \<C>) \<Turnstile>\<^sub>e LET x = SPAWN e\<^sub>c in e" and "(\<V>, \<C>) \<Turnstile>\<^sub>\<rho> \<rho>" by (simp add: accept_state.simps)+
   
   from `(\<V>, \<C>) \<Turnstile>\<^sub>e LET x = SPAWN e\<^sub>c in e`
-  have "(\<V>, \<C>) \<Turnstile>\<^sub>e e\<^sub>c" by (blast intro: accept_exp.cases)
+  have "(\<V>, \<C>) \<Turnstile>\<^sub>e e\<^sub>c" by (blast intro: static_eval.cases)
 
-  have "(\<V>, \<C>) \<Turnstile>\<^sub>\<kappa> \<V> (\<lfloor>e\<^sub>c\<rfloor>) \<Rrightarrow> []" by (simp add: accept_stack.Empty)
+  have "(\<V>, \<C>) \<Turnstile>\<^sub>\<kappa> \<V> (\<lfloor>e\<^sub>c\<rfloor>) \<Rrightarrow> []" by (simp add: static_eval_stack.Empty)
   from \<open>(\<V>, \<C>) \<Turnstile>\<^sub>\<kappa> \<V> (\<lfloor>e\<^sub>c\<rfloor>) \<Rrightarrow> []\<close> \<open>(\<V>, \<C>) \<Turnstile>\<^sub>\<rho> \<rho>\<close> \<open>(\<V>, \<C>) \<Turnstile>\<^sub>e e\<^sub>c\<close> 
   have "(\<V>, \<C>) \<Turnstile>\<^sub>\<sigma> \<langle>e\<^sub>c;\<rho>;[]\<rangle>" by (simp add: accept_state.intros)
 
@@ -1355,7 +1355,7 @@ proof
     assume "(\<E>(\<pi> ;; `x \<mapsto> \<langle>e;\<rho>(x \<mapsto> \<lbrace>\<rbrace>);\<kappa>\<rangle>, \<pi> ;; .x \<mapsto> \<langle>e\<^sub>c;\<rho>;[]\<rangle>)) \<pi>' = Some \<sigma>'"
     and "\<pi>' \<noteq> \<pi> ;; `x" and " \<pi>' \<noteq> \<pi> ;; .x" then
     have "\<E> \<pi>' = Some \<sigma>'" by simp with `(\<V>, \<C>) \<Turnstile>\<^sub>\<E> \<E>`
-    have "(\<V>, \<C>) \<Turnstile>\<^sub>\<sigma> \<sigma>'" by (blast intro: accept_state_pool.cases)
+    have "(\<V>, \<C>) \<Turnstile>\<^sub>\<sigma> \<sigma>'" by (blast intro: static_eval_pool.cases)
   } with `(\<V>, \<C>) \<Turnstile>\<^sub>\<sigma> \<langle>e;\<rho>(x \<mapsto> \<lbrace>\<rbrace>);\<kappa>\<rangle>` and `(\<V>, \<C>) \<Turnstile>\<^sub>\<sigma> \<langle>e\<^sub>c;\<rho>;[]\<rangle>`
   show "\<forall>\<pi>' \<sigma>'. (\<E>(\<pi> ;; `x \<mapsto> \<langle>e;\<rho>(x \<mapsto> \<lbrace>\<rbrace>);\<kappa>\<rangle>, \<pi> ;; .x \<mapsto> \<langle>e\<^sub>c;\<rho>;[]\<rangle>)) \<pi>' = Some \<sigma>' \<longrightarrow> (\<V>, \<C>) \<Turnstile>\<^sub>\<sigma> \<sigma>'" by simp
 qed
@@ -1469,7 +1469,7 @@ proof -
   {
     fix x
     from `(\<V>, \<C>) \<Turnstile>\<^sub>\<rho> \<rho>`
-    have "\<forall>\<omega>. \<rho> x = Some \<omega> \<longrightarrow> {|\<omega>|} \<subseteq> \<V> x" by (simp add: accept_val_env.simps) then
+    have "\<forall>\<omega>. \<rho> x = Some \<omega> \<longrightarrow> {|\<omega>|} \<subseteq> \<V> x" by (simp add: static_eval_env.simps) then
     have "(case \<rho> x of None \<Rightarrow> {} | Some \<omega> \<Rightarrow> {|\<omega>|}) \<subseteq> \<V> x"  by (simp add: option.case_eq_if) then
     have "(\<parallel>\<rho>\<parallel>) x \<subseteq> \<V> x" by (simp add: env_to_abstract_value_env_def)
   } then
@@ -1486,7 +1486,7 @@ theorem accept_pool_to_precise : "
 "
 proof -
   assume "(\<V>, \<C>) \<Turnstile>\<^sub>\<E> \<E>" and "\<E> \<pi> = Some (\<langle>e; \<rho>; \<kappa>\<rangle>)" then
-  have "(\<V>, \<C>) \<Turnstile>\<^sub>\<sigma> \<langle>e; \<rho>; \<kappa>\<rangle>" by (simp add: accept_state_pool.simps) then
+  have "(\<V>, \<C>) \<Turnstile>\<^sub>\<sigma> \<langle>e; \<rho>; \<kappa>\<rangle>" by (simp add: static_eval_pool.simps) then
   have "(\<V>, \<C>) \<Turnstile>\<^sub>\<rho> \<rho>" by (simp add: accept_state.simps) then
   show "\<parallel>\<rho>\<parallel> \<sqsubseteq> \<V>"  by (simp add: accept_env_to_precise)
 qed
@@ -1507,7 +1507,7 @@ proof -
 qed
 
 
-lemma accept_exp_to_pool: "
+lemma static_eval_to_pool: "
   \<lbrakk>
     (\<V>, \<C>) \<Turnstile>\<^sub>e e
   \<rbrakk> \<Longrightarrow>
@@ -1516,15 +1516,15 @@ lemma accept_exp_to_pool: "
 proof -
   assume "(\<V>, \<C>) \<Turnstile>\<^sub>e e"
 
-  have "(\<V>, \<C>) \<Turnstile>\<^sub>\<rho> empty" by (simp add: accept_value_accept_val_env.Any)
-  have "(\<V>, \<C>) \<Turnstile>\<^sub>\<kappa> \<V> (\<lfloor>e\<rfloor>) \<Rrightarrow> []" by (simp add: accept_stack.Empty)
+  have "(\<V>, \<C>) \<Turnstile>\<^sub>\<rho> empty" by (simp add: static_eval_value_static_eval_env.Any)
+  have "(\<V>, \<C>) \<Turnstile>\<^sub>\<kappa> \<V> (\<lfloor>e\<rfloor>) \<Rrightarrow> []" by (simp add: static_eval_stack.Empty)
 
   from `(\<V>, \<C>) \<Turnstile>\<^sub>e e` and `(\<V>, \<C>) \<Turnstile>\<^sub>\<rho> empty` and `(\<V>, \<C>) \<Turnstile>\<^sub>\<kappa> \<V> (\<lfloor>e\<rfloor>) \<Rrightarrow> []`
   have "(\<V>, \<C>) \<Turnstile>\<^sub>\<sigma> \<langle>e; empty; []\<rangle>" by (simp add: accept_state.intros)
 
   have "[[] \<mapsto> \<langle>e; empty; []\<rangle>] [] = Some (\<langle>e; empty; []\<rangle>)" by simp
   with `(\<V>, \<C>) \<Turnstile>\<^sub>\<sigma> \<langle>e; empty; []\<rangle>`
-  show "(\<V>, \<C>) \<Turnstile>\<^sub>\<E> [[] \<mapsto> \<langle>e; empty; []\<rangle>]" by (simp add: accept_state_pool.intros)
+  show "(\<V>, \<C>) \<Turnstile>\<^sub>\<E> [[] \<mapsto> \<langle>e; empty; []\<rangle>]" by (simp add: static_eval_pool.intros)
 qed
 
 
@@ -1541,7 +1541,7 @@ proof -
   and "\<E>' \<pi> = Some (\<langle>e'; \<rho>'; \<kappa>'\<rangle>)"
 
   from `(\<V>, \<C>) \<Turnstile>\<^sub>e e`
-  have "(\<V>, \<C>) \<Turnstile>\<^sub>\<E> [[] \<mapsto> \<langle>e; empty; []\<rangle>]" by (simp add: accept_exp_to_pool)
+  have "(\<V>, \<C>) \<Turnstile>\<^sub>\<E> [[] \<mapsto> \<langle>e; empty; []\<rangle>]" by (simp add: static_eval_to_pool)
 
   from \<open>(\<V>, \<C>) \<Turnstile>\<^sub>\<E> [[] \<mapsto> \<langle>e;Map.empty;[]\<rangle>]\<close> \<open>[[] \<mapsto> \<langle>e;Map.empty;[]\<rangle>] \<rightarrow>* \<E>'\<close> \<open>\<E>' \<pi> = Some (\<langle>e';\<rho>';\<kappa>'\<rangle>)\<close>
   show "\<parallel>\<rho>'\<parallel> \<sqsubseteq> \<V>" by (simp add: accept_pool_sound)
