theory/Dynamic_Com_Topo_Analysis.thy
@@ -2,14 +2,14 @@ theory Dynamic_Com_Topo_Analysis
   imports Main Syntax Dynamic_Semantics
 begin
 
-definition is_send_path :: "state_pool \<Rightarrow> chan \<Rightarrow> control_path \<Rightarrow> bool" where
+definition is_send_path :: "trace_pool \<Rightarrow> chan \<Rightarrow> control_path \<Rightarrow> bool" where
   "is_send_path \<E> c \<pi>\<^sub>y \<equiv> (\<exists> x\<^sub>y x\<^sub>e e\<^sub>n \<kappa> \<rho> x\<^sub>s\<^sub>c x\<^sub>m \<rho>\<^sub>e.
     \<E> \<pi>\<^sub>y = Some (\<langle>LET x\<^sub>y = SYNC x\<^sub>e in e\<^sub>n; \<rho>; \<kappa>\<rangle>) \<and>
     \<rho> x\<^sub>e = Some \<lbrace>Send_Evt x\<^sub>s\<^sub>c x\<^sub>m, \<rho>\<^sub>e\<rbrace> \<and> 
     \<rho>\<^sub>e x\<^sub>s\<^sub>c = Some \<lbrace>c\<rbrace>
   )"
 
-definition is_recv_path :: "state_pool \<Rightarrow> chan \<Rightarrow> control_path \<Rightarrow> bool" where
+definition is_recv_path :: "trace_pool \<Rightarrow> chan \<Rightarrow> control_path \<Rightarrow> bool" where
   "is_recv_path \<E> c \<pi>\<^sub>y \<equiv> (\<exists> x\<^sub>y x\<^sub>e e\<^sub>n \<kappa> \<rho> x\<^sub>r\<^sub>c \<rho>\<^sub>e.
     \<E> \<pi>\<^sub>y = Some (\<langle>LET x\<^sub>y = SYNC x\<^sub>e in e\<^sub>n; \<rho>; \<kappa>\<rangle>) \<and> 
     \<rho> x\<^sub>e = Some \<lbrace>Recv_Evt x\<^sub>r\<^sub>c, \<rho>\<^sub>e\<rbrace> \<and> 
@@ -27,19 +27,19 @@ definition all  :: "(control_path \<Rightarrow> bool) \<Rightarrow> (control_pat
 fun ordered where
   "ordered \<pi>\<^sub>1 \<pi>\<^sub>2 = (prefix \<pi>\<^sub>1 \<pi>\<^sub>2 \<or> prefix \<pi>\<^sub>2 \<pi>\<^sub>1)"
 
-definition one_shot :: "state_pool \<Rightarrow> chan \<Rightarrow> bool" where
+definition one_shot :: "trace_pool \<Rightarrow> chan \<Rightarrow> bool" where
   "one_shot \<E> c \<equiv> all (is_send_path \<E> c) op="
 
 
-definition one_to_one :: "state_pool \<Rightarrow> chan \<Rightarrow> bool" where
+definition one_to_one :: "trace_pool \<Rightarrow> chan \<Rightarrow> bool" where
   "one_to_one \<E> c \<equiv> all (is_send_path \<E> c) ordered \<and> all (is_recv_path \<E> c) ordered"
   
 
-definition fan_out :: "state_pool \<Rightarrow> chan \<Rightarrow> bool" where
+definition fan_out :: "trace_pool \<Rightarrow> chan \<Rightarrow> bool" where
   "fan_out \<E> c \<equiv> all (is_send_path \<E> c) ordered"
   
 
-definition fan_in :: "state_pool \<Rightarrow> chan \<Rightarrow> bool" where
+definition fan_in :: "trace_pool \<Rightarrow> chan \<Rightarrow> bool" where
   "fan_in \<E> c \<equiv> all (is_recv_path \<E> c) ordered"
 
 
