theory/Sound_Traceability.thy
@@ -838,7 +838,7 @@ proof -
   and "\<E> \<pi> = Some (\<langle>e; \<rho>; \<kappa>\<rangle>)"
 
   from `(\<V>, \<C>) \<Turnstile>\<^sub>e e\<^sub>0`
-  have "(\<V>, \<C>) \<Turnstile>\<^sub>\<E> [[] \<mapsto> \<langle>e\<^sub>0; empty; []\<rangle>]" by (simp add: accept_exp_to_pool)
+  have "(\<V>, \<C>) \<Turnstile>\<^sub>\<E> [[] \<mapsto> \<langle>e\<^sub>0; empty; []\<rangle>]" by (simp add: static_eval_to_pool)
 
   from \<open>(\<V>, \<C>) \<Turnstile>\<^sub>\<E> [[] \<mapsto> \<langle>e\<^sub>0;Map.empty;[]\<rangle>]\<close> \<open>\<E> \<pi> = Some (\<langle>e;\<rho>;\<kappa>\<rangle>)\<close> \<open>[[] \<mapsto> \<langle>e\<^sub>0; empty; []\<rangle>] \<rightarrow>* \<E>\<close>
   show "\<V> \<turnstile> e\<^sub>0 \<down> \<pi> \<mapsto> e" using isnt_traceable_sound' by blast
